fixpoint

src/pca.lean
@@ -14,106 +14,102 @@ infixl ` ⬝ ` := partial_magma.mul
 
 infix ` ↓= `:50 := λ x y, x = some y
 
-instance pm_mul {α : Type u} [c : partial_magma α] : has_mul (option α) := {mul := @partial_magma.mmul _ c}
-instance a_to_option_a {α : Type u} : has_coe α (option α) := ⟨some⟩
 
-/- Partial Computability Algebla -/
+
+instance pm_mul {α : Type u} [c : partial_magma α] : has_mul (option α) := {mul := @partial_magma.mmul _ c}
+
+/- Partial Combinatory Algebra -/
 class pca (α : Type u) extends partial_magma α :=
 (k : α)
 (ktot : ∀ x, option.is_some (k ⬝ x))
-(hk : ∀ x y, k ⬝ x * (some y) = some x)
+(k_constant : ∀ x y : α, k ⬝ x * y = x)
 (s : α)
 (stot : ∀ x y : α, option.is_some (s ⬝ x * y))
-(hs : ∀ x y z : α, s ⬝ x * y * z = (x ⬝ z) * (y ⬝ z))
+(s_substitution : ∀ x y z : α, s ⬝ x * y * z = (x ⬝ z) * (y ⬝ z))
+
+def pca.equiv {α : Type u} [partial_magma α] (a b : option α) : Prop := ∀ x, a * x = b * x
+infix ` ≃ `:50 := pca.equiv 
 
 namespace pca
 
 variables {α : Type u}
 
-@[simp] lemma kh_ [c : pca α] : ∀ x y : α, k ⬝ x * (some y) = some x := c.hk
-@[simp] lemma sh_ [c : pca α] : ∀ x y z : α, s ⬝ x * (some y) * (some z) = (x ⬝ z) * (y ⬝ z) := c.hs
+@[simp] lemma k_constant_ [c : pca α] : ∀ x y : α, k ⬝ x * (some y) = some x := c.k_constant
+@[simp] lemma s_substitution_ [c : pca α] : ∀ x y z : α, s ⬝ x * (some y) * (some z) = (x ⬝ z) * (y ⬝ z) := c.s_substitution
 
-def i' [pca α] : option α := s ⬝ k * (some k)
-
-lemma i'_defined [pca α] : option.is_some (i' : option α) = tt := stot k k
-
-def i [pca α] : α := option.get i'_defined
-
-@[simp]
-lemma i'_ident [pca α] (x : α) : i' * (some x) ↓= x := 
-by { calc
-    i' * some x = k ⬝ x * k ⬝ x                        : by { unfold i', simp }
-    ...         = k ⬝ x * (some (option.get (ktot x))) : by { simp }
-    ...         = some x                               : by { simp only [kh_] } }
+def i [pca α] : α := option.get (stot k k)
 
 @[simp]
 lemma i_ident [pca α] (x : α) : i ⬝ x ↓= x :=
 begin
-  have e : i' = some i, { unfold i, simp },
+  have e : s ⬝ k * (some k) = some i, { unfold i, simp, refl },
   calc
-    i ⬝ x = i' * (some x) : by { rw e, exact rfl }
-    ...   = some x        : by { exact i'_ident _ },
+    i ⬝ x = (s ⬝ k * (some k)) * (some x)        : by { rw e, exact rfl }
+    ...   = k ⬝ x * k ⬝ x                        : by { simp }
+    ...   = k ⬝ x * (some (option.get (ktot x))) : by { simp }
+    ...   = some x                               : by { simp only [k_constant_] }
 end
 
-
-inductive lambda
+inductive lambda (α : Type u) [pca α]
 | var : ℕ → lambda
-| K : lambda
-| S : lambda
-| I : lambda
+| com : α → lambda
 | app : lambda → lambda → lambda
+instance lambda_mul (α : Type u) [pca α] : has_mul (lambda α) := ⟨lambda.app⟩
 
 open lambda
 
-local infixl ` *ₗ `:60 := app
-
-def lam : ℕ → lambda → lambda
-| x (var y) := if x = y then I else K *ₗ var y
-| x K := K *ₗ K
-| x S := K *ₗ S
-| x I := K *ₗ I
-| x (l *ₗ k) := S *ₗ (lam x l) *ₗ (lam x k)
+def lam [pca α] : ℕ → lambda α → lambda α
+| x (var y) := if x = y then (com i) else (com k) * var y
+| x (com c) := com k * com c
+| x (l * k) := com s * (lam x l) * (lam x k)
 notation `Λ`x`,` := lam x 
 
-#check @lam
-
-#check Λ 0, K *ₗ (var 0)
-
-def l_to_pca [pca α] : lambda → option α
+def l_to_pca [pca α] : lambda α → option α
 | (var x) := some k
-| K := some k
-| S := some s
-| I := some i
-| (l *ₗ k) := (l_to_pca l) * (l_to_pca k)
+| (com c) := some c
+| (l * k) := (l_to_pca l) * (l_to_pca k)
 
-instance lambda_to_pca {α : Type u} [pca α] : has_coe lambda (option α) := ⟨l_to_pca⟩ 
+instance lambda_to_pca {α : Type u} [pca α] : has_coe (lambda α) (option α) := ⟨l_to_pca⟩ 
 
-#check congr_arg coe
-
-lemma mmul_some_some [pca α] (x y : α) : (some x) * (some y) = x ⬝ y := rfl
-
-lemma lambda_defined [pca α] : ∀ (e : lambda) (n : ℕ) , option.is_some (l_to_pca (Λ n, e) : option α) :=
-begin
-  intros e n,
-  induction e,
-  { cases (eq.decidable n e),
-    { have he : Λ n, (var e) = K *ₗ var e, { simp [lam], intros, contradiction },
+lemma lambda_defined [c : pca α] : ∀ (n : ℕ) (e : lambda α), option.is_some (l_to_pca (Λ n, e) : option α)
+| n (var e) := begin
+    cases (eq.decidable n e),
+    { have he : (Λ n, (var e) : @lambda _ c) = com k * var e, { simp [lam], intros, contradiction },
       rw he,
-      exact ktot _,  },
-    { have he : Λ n, (var e) = I, { simp [lam], intros, contradiction },
+      exact ktot _ },
+    { have he : (Λ n, (var e) : @lambda _ c) = com i, { simp [lam], intros, contradiction },
       rw he,
-      exact rfl } },
-  { exact ktot _ },
-  { exact ktot _ },
-  { exact ktot _ },
-  { simp [lam, l_to_pca], 
-    let a := option.get e_ih_ᾰ,
-    let b := option.get e_ih_ᾰ_1,
-    have ha : l_to_pca (Λ n, e_ᾰ) = some a, { simp },
-    have hb : l_to_pca (Λ n, e_ᾰ_1) = some b, { simp },
+      exact rfl, }
+  end
+| n (com c) := ktot c
+| n (l * m) := begin
+    simp [lam, l_to_pca], 
+    let a := option.get (lambda_defined n l),
+    let b := option.get (lambda_defined n m),
+    have ha : l_to_pca (Λ n, l) = some a, { simp },
+    have hb : l_to_pca (Λ n, m) = some b, { simp },
     rw [ha, hb],
-    exact stot _ _ }
+    exact stot a b
+  end 
+
+def dapp [pca α] : lambda α := Λ 0, (Λ 1, (Λ 2, (var 0) * ((var 1) * (var 1)) * (var 2)))
+
+
+def fixpoint [pca α] : α := option.get (lambda_defined 0 (dapp * (var 0) *(dapp * (var 0))))
+def fixpoint' [pca α] : option α := l_to_pca (Λ 0, dapp * (var 0) *(dapp * (var 0)))
+
+theorem kleene_fixpoint [c : pca α] (f : α) :
+  fixpoint ⬝ f ≃ f * (fixpoint ⬝ f) :=
+begin
+  have e : l_to_pca (Λ 0, (dapp * (var 0) * (dapp * (var 0)))) = some (@fixpoint _ c),
+  { unfold fixpoint, simp },
+  intros x,
+  calc
+    fixpoint ⬝ f * x = (l_to_pca (Λ 0, (dapp * (var 0) * (dapp * (var 0))))) * (some f) * x : by { rw e, exact rfl }
+    ...              = (l_to_pca (dapp * (com f) * (dapp * (com f)))) * x : by { simp [lam, l_to_pca],  }
+    ...              = f * fixpoint ⬝ f * x : by sorry
 end
+
 
 end pca
 
